# 均匀球体对球体外物体的万有引力等效于位于球心处的质点
$$
\begin{aligned}
\cos\alpha &= \frac{D-z}{\sqrt{x^2+y^2+(D-z)^2}} \\
&= \frac{D-r\cos\phi}{\sqrt{r^2\sin^2\phi\cos^2\theta
 +r^2\sin^2\phi\sin^2\theta+D^2-2rD\cos\phi+r^2\cos^2\phi}} \\
&= \frac{D-r\cos\phi}{\sqrt{r^2+D^2-2rD\cos\phi}}
\end{aligned}
$$
$$
\begin{aligned}
F &= \iiint\frac{Gm\rho\text{d}V}{x^2+y^2+(D-z)^2}\cos\alpha \\
&= Gm\rho\iiint\frac{r^2\sin\phi(D-r\cos\phi)}
{(r^2+D^2-2rD\cos\phi)^{\frac{3}{2}}}\text{d}V
\end{aligned}
$$
令
$$
\begin{aligned}
A(\phi) &= r^2\sin\phi(D-r\cos\phi) \\
B(\phi) &= r^2+D^2-2rD\cos\phi
\end{aligned}
$$
则
$$
\begin{aligned}
\frac{\text{d}B(\phi)}{\text{d}\phi} &= 2rD\sin\phi \\
A(\phi) &= r^2\sin\phi(D-r\cos\phi) \\
&= \frac{r(D-r\cos\phi)}{2D}\frac{\text{d}B(\phi)}{\text{d}\phi} \\
&= \frac{r(B(\phi)+D^2-r^2)}{4D^2}\frac{\text{d}B(\phi)}{\text{d}\phi} \\
\end{aligned}
$$
于是
$$
\begin{aligned}
& \int\frac{B(\phi)+D^2-r^2}{B^{\frac{3}{2}}(\phi)}\text{d}B(\phi) \\
=& -2\int(B(\phi)+D^2-r^2)\text{d}B^{-\frac{1}{2}}(\phi) \\
=& -2\left[\sqrt{B(\phi)}+\frac{D^2-r^2}{\sqrt{B(\phi)}}\right]
 +2\int B^{-\frac{1}{2}}(\phi)\text{d}B(\phi) \\
=& -2\left[\sqrt{B(\phi)}+\frac{D^2-r^2}{\sqrt{B(\phi)}}\right]+4\sqrt{B(\phi)} \\
=& 2\sqrt{B(\phi)}-2\frac{D^2-r^2}{\sqrt{B(\phi)}} \\
\end{aligned}
$$
加入上下限
$$
\begin{aligned}
\sqrt{B(0)} =& \sqrt{r^2+D^2-2rD}=D-r \\
\sqrt{B(\pi)} =& \sqrt{r^2+D^2+2rD}=D+r \\
\int_0^{\pi}\frac{B(\phi)+D^2-r^2}{B^{\frac{3}{2}}(\phi)}\text{d}B(\phi)
=& 2\left[\sqrt{B(\phi)}-\frac{D^2-r^2}{\sqrt{B(\phi)}}\right]_0^{\pi} \\
=& 2[(D+r)-(D-r)]-2[(D-r)-(D+r)] \\
=& 8r
\end{aligned}
$$
代入$F$
$$
\begin{aligned}
F =& Gm\rho\iiint\frac{r^2\sin\phi(D-r\cos\phi)}
{(r^2+D^2-2rD\cos\phi)^{\frac{3}{2}}}\text{d}V \\
=& Gm\rho\int_0^{2\pi}\int_0^{\pi}\int_0^{R}\frac{r^2\sin\phi(D-r\cos\phi)}
{(r^2+D^2-2rD\cos\phi)^{\frac{3}{2}}}\text{d}r\text{d}\phi\text{d}\theta \\
=& 2\pi Gm\rho\int_0^{\pi}\int_0^{R}\frac{r^2\sin\phi(D-r\cos\phi)}
{(r^2+D^2-2rD\cos\phi)^{\frac{3}{2}}}\text{d}r\text{d}\phi \\
=& 2\pi Gm\rho\int_0^{R}\int_0^{\pi}\int\frac{A(\phi)}
 {B^{\frac{3}{2}}(\phi)}\text{d}\phi\text{d}r \\
=& 2\pi Gm\rho\int_0^{R}\int_0^{\pi}\frac{r(B(\phi)+D^2-r^2)}
 {4D^2B^{\frac{3}{2}}(\phi)}\text{d}B(\phi)\text{d}r \\
=& \frac{\pi Gm\rho r}{2D^2}\int_0^{R}r\int_0^{\pi}\frac{B(\phi)+D^2-r^2}
 {B^{\frac{3}{2}}(\phi)}\text{d}B(\phi)\text{d}r \\
=& \frac{\pi Gm\rho}{2D^2}\int_0^{R}8r^2\text{d}r \\
=& \frac{4\pi Gm\rho}{D^2}\frac{R^3}{3} \\
=& \frac{4\pi GmR^3}{3D^2}\frac{M}{\frac{4}{3}\pi R^3} \\
=& \frac{GMm}{D^2}
\end{aligned}
$$

# 均匀球壳对球壳内任意一点的万有引力合力为0
积分
$$
\int_0^{\pi}\frac{B(\phi)+D^2-r^2}{B^{\frac{3}{2}}(\phi)}\text{d}B(\phi)
$$
中，由于$D\le r$，所以$\sqrt{B(0)}=\sqrt{r^2+D^2-2rD}=r-D$，此时
$$
\begin{aligned}
\int_0^{\pi}\frac{B(\phi)+D^2-r^2}{B^{\frac{3}{2}}(\phi)}\text{d}B(\phi)
=& 2\left[\sqrt{B(\phi)}-\frac{D^2-r^2}{\sqrt{B(\phi)}}\right]_0^{\pi} \\
=& 2[(D+r)-(D-r)]-2[(r-D)+(r+D)] \\
=& 0
\end{aligned}
$$
代入$F$
$$
\begin{aligned}
F =& Gm\rho\int_0^{2\pi}\int_0^{\pi}\int_{R_1}^{R_2}\frac{r^2\sin\phi(D-r\cos\phi)}
{(r^2+D^2-2rD\cos\phi)^{\frac{3}{2}}}\text{d}r\text{d}\phi\text{d}\theta \\
=& \frac{\pi Gm\rho r}{2D^2}\int_{R_1}^{R_2}r\int_0^{\pi}\frac{B(\phi)+D^2-r^2}
 {B^{\frac{3}{2}}(\phi)}\text{d}B(\phi)\text{d}r \\
=& 0
\end{aligned}
$$

